Reduce DisjointTokens-related invariants to more basic ones

Wavelet/Semantics/Defs.lean
@@ -510,6 +510,12 @@ instance [Arity Op] : IsRefl (Semantics Op V m n) IORestrictedSimilarity where
 instance [Arity Op] : IsTrans (Semantics Op V m n) IORestrictedSimilarity where
   trans _ _ _ := .trans
 
+/-- An invariant holds for all states reachable via the given set of labels. -/
+def Lts.IsInvariantForAt
+  (lts : Lts C E) (Labels : E → Prop) (P : C → Prop) (c : C) : Prop :=
+  ∀ {c' tr}, lts.Star c tr c' → (∀ {l}, l ∈ tr → Labels l) → P c'
+
+/-- An invariant holds for all state reachable from the given state. -/
 def Lts.IsInvariantAt
   (lts : Lts C E) (P : C → Prop) (c : C) : Prop :=
   ∀ {c' tr}, lts.Star c tr c' → P c'
@@ -541,6 +547,23 @@ theorem Lts.IsInvariantAt.by_induction
   | refl => exact hbase
   | tail pref tail ih => exact hstep (ih hbase) tail
 
+theorem Lts.IsInvariantForAt.by_induction
+  {lts : Lts C E}
+  {Labels : E → Prop}
+  {P : C → Prop}
+  {c : C}
+  (hbase : P c)
+  (hstep : ∀ {c₁ c₂ l},
+    P c₁ → Labels l → lts.Step c₁ l c₂ → P c₂) :
+  lts.IsInvariantForAt Labels P c := by
+  intros c' tr hstar hlabels
+  induction hstar with
+  | refl => exact hbase
+  | tail pref tail ih =>
+    simp at hlabels
+    have := ih hbase (λ hl => hlabels (.inl hl))
+    exact hstep this (hlabels (.inr rfl)) tail
+
 /-- Prove an invariant by strong induction. -/
 theorem Lts.IsInvariantAt.by_strong_induction
   {lts : Lts C E}
@@ -556,10 +579,33 @@ theorem Lts.IsInvariantAt.by_strong_induction
   | tail pref tail ih =>
     exact hstep pref (ih hbase hstep) tail
 
+theorem Lts.IsInvariantForAt.by_strong_induction
+  {lts : Lts C E}
+  {Labels : E → Prop}
+  {P : C → Prop}
+  {c : C}
+  (hbase : P c)
+  (hstep : ∀ {c₁ c₂ l tr},
+    lts.Star c tr c₁ → (∀ {l}, l ∈ tr → Labels l) →
+    P c₁ → Labels l → lts.Step c₁ l c₂ → P c₂) :
+  lts.IsInvariantForAt Labels P c := by
+  intros c' tr hstar hlabels
+  induction hstar with
+  | refl => exact hbase
+  | tail pref tail ih =>
+    simp at hlabels
+    grind only [cases Or]
+
 theorem Lts.IsInvariantAt.base
   {lts : Lts C E}
   {P : C → Prop} {c : C}
   (hinv : lts.IsInvariantAt P c) : P c := hinv .refl
+
+theorem Lts.IsInvariantForAt.base
+  {lts : Lts C E}
+  {Labels : E → Prop}
+  {P : C → Prop} {c : C}
+  (hinv : lts.IsInvariantForAt Labels P c) : P c := hinv .refl (by simp)
 
 theorem Lts.IsInvariantAt.unfold
   {lts : Lts C E}
@@ -571,8 +617,27 @@ theorem Lts.IsInvariantAt.unfold
     hinv (Lts.Star.tail .refl hstep),
     by
       intros c'' tr hstar
+      exact hinv (hstar.prepend hstep)⟩
+
+theorem Lts.IsInvariantForAt.unfold
+  {lts : Lts C E}
+  {Labels : E → Prop}
+  {P : C → Prop} {c c' : C} {l : E}
+  (hinv : lts.IsInvariantForAt Labels P c)
+  (hstep : lts.Step c l c')
+  (hl : Labels l) :
+    P c' ∧ lts.IsInvariantForAt Labels P c'
+  := ⟨
+    hinv (Lts.Star.tail .refl hstep) (by simp [hl]),
+    by
+      intros c'' tr hstar htr
       exact hinv (hstar.prepend hstep)
-  ⟩
+        (by
+          intros l' hl'
+          simp at hl'
+          cases hl' <;> rename_i h
+          · subst h; exact hl
+          · exact htr h)⟩
 
 theorem Lts.IsInvariantAt.map_step
   {lts₁ : Lts C E₁}
@@ -583,6 +648,45 @@ theorem Lts.IsInvariantAt.map_step
   intros c tr hsteps
   have ⟨_, hsteps'⟩ := hsteps.map_hetero_step hmap
   exact hinv hsteps'
+
+theorem Lts.IsInvariantForAt.map_step
+  {lts₁ : Lts C E₁}
+  {lts₂ : Lts C E₂}
+  {Labels₁ : E₁ → Prop}
+  {Labels₂ : E₂ → Prop}
+  {P : C → Prop}
+  (hmap : ∀ {c c' l₂},
+    Labels₂ l₂ → lts₂.Step c l₂ c' → ∃ l₁, Labels₁ l₁ ∧ lts₁.Step c l₁ c')
+  (hinv : lts₁.IsInvariantForAt Labels₁ P c) :
+    lts₂.IsInvariantForAt Labels₂ P c := by
+  intros c₁ tr hsteps htr
+  have ⟨tr', htr', hsteps'⟩ := hsteps.map_hetero_step_alt hmap htr
+  exact hinv hsteps' htr'
+
+/-- Converts `IsInvariantForAt` to `IsInvariantAt` when the
+label restriction always holds in the LTS. -/
+theorem Lts.IsInvariantForAt.to_inv_at
+  {lts : Lts C E}
+  {Labels : E → Prop}
+  {P : C → Prop}
+  (hl : ∀ {c l c'}, lts.Step c l c' → Labels l)
+  (hinv : lts.IsInvariantForAt Labels P c) : lts.IsInvariantAt P c := by
+  intros c₁ tr hsteps
+  induction hsteps using Lts.Star.reverse_induction with
+  | refl => exact hinv .refl (by simp)
+  | head head tail ih =>
+    apply ih
+    exact (hinv.unfold head (hl head)).2
+
+theorem Lts.IsInvariantForAt.imp_labels
+  {lts : Lts C E}
+  {Labels₁ Labels₂ : E → Prop}
+  {P : C → Prop}
+  (himp : ∀ l, Labels₂ l → Labels₁ l)
+  (hinv : lts.IsInvariantForAt Labels₁ P c) :
+    lts.IsInvariantForAt Labels₂ P c := by
+  intros c' tr hstar hlabels
+  exact hinv hstar (by intros l hl; exact himp l (hlabels hl))
 
 theorem Lts.IsInvariantAt.imp
   {lts : Lts C E}
