Wavelet/Determinacy/DisjointTokens.lean
@@ -1,7 +1,10 @@
 import Wavelet.Seq.Fn
 import Wavelet.Dataflow.Proc
 import Wavelet.Dataflow.AffineChan
+
 import Wavelet.Determinacy.Defs
+import Wavelet.Determinacy.Convert
+import Wavelet.Determinacy.Determinism
 
 /-! Definitions and lemmas about configurations having a disjoint set of tokens. -/
 
@@ -72,22 +75,99 @@ namespace Wavelet.Determinacy
 
 open Semantics Dataflow
 
-theorem Config.DisjointTokens.inv
+theorem proc_guarded_inv_aff
+  [Arity Op] [PCM T]
+  [DecidableEq χ]
+  [InterpConsts V]
+  {opSpec : OpSpec Op V T}
+  {ioSpec : IOSpec V T m n}
+  {s : ConfigWithSpec opSpec χ m n}
+  (haff : s.proc.AffineChan) :
+    (Config.GuardStep opSpec ioSpec).IsInvariantAt (·.proc.AffineChan) s
+  := by
+  simp [Config.GuardStep]
+  have : (Config.GuardStep opSpec ioSpec).IsInvariantAt _ _ :=
+    (Lts.GuardStep.map_inv (P := opSpec.Guard ioSpec) (haff.inv))
+  intros s' tr hsteps
+  exact this hsteps
+
+theorem proc_indexed_guarded_inv_aff
+  [Arity Op] [PCM T]
+  [DecidableEq χ]
+  [InterpConsts V]
+  {opSpec : OpSpec Op V T}
+  {ioSpec : IOSpec V T m n}
+  {s : ConfigWithSpec opSpec χ m n}
+  (haff : s.proc.AffineChan) :
+    (Config.IdxGuardStep opSpec ioSpec).IsInvariantAt (·.proc.AffineChan) s
+  := by
+  have : (Config.GuardStep opSpec ioSpec).IsInvariantAt _ _ := proc_guarded_inv_aff haff
+  have : (Config.IdxGuardStep opSpec ioSpec).IsInvariantAt _ _ := this.map_step (λ hstep => by
+    simp [Lts.Step] at hstep
+    exact ⟨_, hstep.to_guarded⟩)
+  intros s' tr hsteps
+  exact this hsteps
+
+theorem proc_interp_guarded_inv_aff
+  [Arity Op] [PCM T]
+  [DecidableEq χ]
+  [InterpConsts V]
+  [opInterp : OpInterp Op V]
+  {opSpec : OpSpec Op V T}
+  {ioSpec : IOSpec V T m n}
+  {s : ConfigWithSpec opSpec χ m n × opInterp.S}
+  (haff : s.1.proc.AffineChan) :
+    (Config.InterpGuardStep opSpec ioSpec).IsInvariantAt (·.1.proc.AffineChan) s
+  := by
+  simp [Config.InterpGuardStep]
+  have : (Config.InterpGuardStep opSpec ioSpec).IsInvariantAt _ _ :=
+    (Lts.InterpStep.map_inv
+      (lts' := opInterp.lts)
+      (Inv := λ (s : ConfigWithSpec opSpec χ m n) => s.proc.AffineChan)
+      (Lts.GuardStep.map_inv (P := opSpec.Guard ioSpec) (haff.inv)))
+  intros s' tr hsteps
+  exact this hsteps
+
+theorem proc_indexed_interp_guarded_inv_aff
+  [Arity Op] [PCM T]
+  [DecidableEq χ]
+  [InterpConsts V]
+  [opInterp : OpInterp Op V]
+  {opSpec : OpSpec Op V T}
+  {ioSpec : IOSpec V T m n}
+  {s : ConfigWithSpec opSpec χ m n × opInterp.S}
+  (haff : s.1.proc.AffineChan) :
+    (Config.IdxInterpGuardStep opSpec ioSpec).IsInvariantAt (·.1.proc.AffineChan) s
+  := by
+  have : (Config.InterpGuardStep opSpec ioSpec).IsInvariantAt _ _ := proc_interp_guarded_inv_aff haff
+  have : (Config.IdxInterpGuardStep opSpec ioSpec).IsInvariantAt _ _ := this.map_step (λ hstep => by
+    simp [Lts.Step] at hstep
+    exact ⟨_, hstep.to_interp_guarded⟩)
+  intros s' tr hsteps
+  exact this hsteps
+
+/--
+`Config.DisjointTokens` is an invariant of a guarded `Proc` semantics,
+when restricted to non-input labels.
+-/
+theorem Config.DisjointTokens.guarded_inv
   [Arity Op] [PCM T] [DecidableEq χ]
   [InterpConsts V]
-  {s : Dataflow.Config Op χ (V ⊕ T) m n}
+  {opSpec : OpSpec Op V T}
+  {ioSpec : IOSpec V T m n}
+  {s : Dataflow.ConfigWithSpec opSpec χ m n}
   (haff : s.proc.AffineChan)
   (hdisj : s.DisjointTokens) :
-    Config.Step.IsInvariantAt Config.DisjointTokens s
+    (Config.GuardStep opSpec ioSpec).IsInvariantForAt
+      (¬ ·.isInput)
+      Config.DisjointTokens s
   := by
   sorry
 
 /--
-`Config.DisjointTokens` is a state invariant of a guarded `Proc` semantics.
-
-TODO: this requires the `opSpec` to be frame preserving.
+`Config.DisjointTokens` is an invariant of an interpreted and guarded `Proc` semantics.
 -/
-theorem Config.DisjointTokens.guarded_interp_inv
+theorem Config.DisjointTokens.interp_guarded_inv
   [Arity Op] [PCM T] [DecidableEq χ]
   [InterpConsts V]
   [opInterp : OpInterp Op V]
@@ -96,9 +176,72 @@ theorem Config.DisjointTokens.guarded_interp_inv
   {s : Dataflow.ConfigWithSpec opSpec χ m n × opInterp.S}
   (haff : s.1.proc.AffineChan)
   (hdisj : s.1.DisjointTokens) :
-    (Config.InterpGuardStep opSpec ioSpec).IsInvariantAt
+    (Config.InterpGuardStep opSpec ioSpec).IsInvariantForAt
+      (¬ ·.isInput)
       (Config.DisjointTokens ·.1) s
   := by
-  sorry
+  intros s' tr hsteps htr
+  suffices h :
+    s'.fst.proc.AffineChan ∧
+    s'.fst.DisjointTokens by
+    with_reducible
+    exact h.2
+  induction hsteps with
+  | refl => exact ⟨haff, hdisj⟩
+  | tail pref tail ih =>
+    rename_i s tr₁ s₁ l₂ s₂
+    simp at htr
+    have ⟨haff', hdisj'⟩ := ih haff hdisj
+      (by
+        intros l hmem
+        simp [htr (.inl hmem)])
+    have hinv_aff : (Config.GuardStep opSpec ioSpec).IsInvariantAt _ _ :=
+      proc_guarded_inv_aff haff'
+    have hinv_disj : (Config.GuardStep opSpec ioSpec).IsInvariantForAt _ _ _ :=
+      Config.DisjointTokens.guarded_inv haff' hdisj'
+    simp [Config.InterpGuardStep] at tail
+    cases tail with
+    | step_tau tail
+    | step_output tail
+    | step_yield tail =>
+      exact ⟨
+        (hinv_aff.unfold tail).1,
+        (hinv_disj.unfold tail (by simp)).1,
+      ⟩
+    | step_input =>
+      have := htr (.inr rfl)
+      simp at this
+
+/--
+Converts the previous invariant results to `Config.IdxInterpGuardStep`
+-/
+theorem Config.DisjointTokens.indexed_interp_guarded_inv
+  [Arity Op] [PCM T] [DecidableEq χ]
+  [InterpConsts V]
+  [opInterp : OpInterp Op V]
+  {opSpec : OpSpec Op V T}
+  {ioSpec : IOSpec V T m n}
+  {s : Dataflow.ConfigWithSpec opSpec χ m n × opInterp.S}
+  (haff : s.1.proc.AffineChan)
+  (hdisj : s.1.DisjointTokens) :
+    (Config.IdxInterpGuardStep opSpec ioSpec).IsInvariantAt
+      (Config.DisjointTokens ·.1) s
+  := by
+  with_reducible
+  have : (Config.InterpGuardStep opSpec ioSpec).IsInvariantForAt _ _ _ :=
+    Config.DisjointTokens.interp_guarded_inv haff hdisj
+  have := this.imp_labels
+    (Labels₂ := λ (l : Label _ V m n) => l.isSilent)
+    (by intros l; cases l <;> simp)
+  have : (Config.IdxInterpGuardStep opSpec ioSpec).IsInvariantForAt _ _ _ :=
+    this.map_step
+      (Labels₂ := λ _ => True)
+      (by
+        intros c c' l hl hstep
+        have hstep' := Config.IdxInterpGuardStep.to_interp_guarded hstep
+        have := proc_indexed_interp_guarded_step_label hstep
+        simp [this] at hstep'
+        exact ⟨_, by simp, hstep'⟩)
+  exact Lts.IsInvariantForAt.to_inv_at (by simp) this
 
 end Wavelet.Determinacy
